NBE.lean
@@ -10,3 +10,4 @@ import NBE.SingleSortImp.BetaEtaNormalizing
 import NBE.SingleSortImp.BetaEtaCons
 import NBE.SingleSortImp.RealPresheaf
 import NBE.SingleSortImp.StrongBeta
+import NBE.SingleSortImp.ExpCounterExample
