NBE/SingleSortImp/ExpCounterExample.lean
@@ -1,0 +1,217 @@
+import NBE.SingleSortImp.BetaEta
+
+namespace SingleSortImp.CounterExample
+
+def Stronger (Γ' Γ: Context): Prop := exists Δ, Γ' = Δ ++ Γ
+
+def Stronger.refl {Γ: Context}: Stronger Γ Γ
+:= by
+  exists []
+
+def Stronger.comp {Γ'' Γ' Γ: Context}:
+  Stronger Γ' Γ -> Stronger Γ'' Γ' -> Stronger Γ'' Γ
+:= by
+  rintro ⟨Δ, E⟩ ⟨Δ', E'⟩
+  exists (Δ' ++ Δ)
+  simp [E', E]
+
+notation Γ' " >> " Γ => Stronger Γ' Γ
+
+
+def Stronger.length {Γ' Γ: Context} (_: Γ' >> Γ): Nat := Γ'.length - Γ.length
+def Stronger.diff {Γ' Γ: Context} (r: Γ' >> Γ): Context := Γ'.take (Stronger.length r)
+
+
+@[simp]
+theorem Stronger.diff_length {Γ' Γ: Context} (r: Γ' >> Γ):
+  r.length = Γ'.length - Γ.length
+:= by
+  simp [Stronger.length]
+
+
+theorem Stronger.diff_eq {Γ' Γ: Context} (r: Γ' >> Γ):
+  Γ' = r.diff ++ Γ
+:= by
+  unfold Stronger.diff
+  simp [Stronger.length]
+  rcases r with ⟨Δ, E⟩
+  simp [E]
+
+
+structure Presheaf where
+  obj: Context -> Type
+  map {Γ' Γ: Context} (r: Γ' >> Γ): obj Γ -> obj Γ'
+  map_id {Γ: Context}: forall {x: obj Γ}, map .refl x = x
+  map_comp {Γ'' Γ' Γ: Context} {r': Γ'' >> Γ'} {r: Γ' >> Γ}:
+     forall {x: obj Γ}, map r' (map r x) = map (Stronger.comp r r') x
+
+
+structure NatTrans (F G: Presheaf) where
+  trans {Γ: Context}: F.obj Γ -> G.obj Γ
+  nat {Γ' Γ: Context} (r: Γ' >> Γ):
+    forall {x: F.obj Γ}, trans (F.map r x) = G.map r (trans x)
+
+
+def NF (T: Ty): Presheaf where
+  obj Γ := {t: Tm // Tm.NF Γ t T}
+  map {Γ' Γ: Context} r := by
+    rintro ⟨t, N⟩
+    exists (t.up 0 r.length)
+    simp
+    have E := r.diff_eq
+    generalize r.diff = Δ at *
+    clear r
+    simp [E]
+    apply Tm.NF.weaken_app
+    exact N
+  map_id {Γ: Context} := by
+    rintro ⟨t, N⟩
+    simp
+  map_comp {Γ'' Γ' Γ: Context} := by
+    rintro ⟨Δ', E'⟩ ⟨Δ, E⟩
+    rintro ⟨t, N⟩
+    simp_all
+    congr
+    omega
+
+
+theorem headType_atomic {Γ t T} (N: Tm.NE Γ t T):
+  N.headType = .Atom -> t = .var t.headVar
+:= by
+  intro E
+  induction t generalizing T
+  case var x =>
+    simp [Tm.headVar]
+  case abs =>
+    cases N
+  case app t1 t2 IH1 IH2 =>
+    simp [Tm.NE.headType, Tm.headVar] at E
+    cases N with | app N _ =>
+    specialize IH1 N E
+    rewrite [IH1] at N
+    cases N with | var N =>
+    have K: t1.headVar < Γ.length := by
+      apply FinMap.lookup_some_lt N
+    rewrite [FinMap.lookup_lt_some K] at N
+    rewrite [E] at N
+    cases N
+
+
+theorem NF_singleton:
+  forall x: (NF (Ty.Atom.imp .Atom)).obj [], x.val = Tm.abs (Tm.var 0)
+:= by
+  rintro ⟨t, N⟩
+  simp
+  cases N with | abs N =>
+  rename_i t
+  cases N with | atom N =>
+  have H := N.headVar_lt
+  simp at H
+  have A: N.headType = .Atom := by
+    simp [Tm.NE.headType]
+  replace N := headType_atomic N A
+  rewrite [H] at N
+  simp_all
+
+
+def P := NF (Ty.Atom)
+
+
+def η_id: NatTrans P P where
+  trans {Γ} := id
+  nat {Γ' Γ} r := by
+    simp
+
+
+def η_trans (Γ: Context) (t: Tm): Tm :=
+  match t with
+  | .app (.var f) _ =>
+    match Γ.lookup f with
+    | some (Ty.imp (Ty.imp Ty.Atom Ty.Atom) Ty.Atom) =>
+      .app (.var f) (.abs (.var 0))
+    | _ => t
+  | _ => t
+
+
+def η: NatTrans P P where
+  trans {Γ} := by
+    rintro ⟨t, N⟩
+    exists η_trans Γ t
+    simp [η_trans]
+    split
+    . split
+      . apply Tm.NF.atom
+        apply Tm.NE.app
+        . apply Tm.NE.var
+          assumption
+        . apply Tm.NF.abs
+          apply Tm.NF.atom
+          apply Tm.NE.var
+          simp
+      . exact N
+    . exact N
+  nat {Γ' Γ} r := by
+    rintro ⟨t, N⟩
+    simp only [P, NF]
+    apply Subtype.ext
+    simp
+    cases t with
+    | var x | abs =>
+      simp [η_trans, Tm.up]
+    | app t1 t2 =>
+      cases t1 with
+      | app | abs =>
+        simp [η_trans, Tm.up]
+      | var f =>
+        generalize E: Γ.lookup f = T
+        have K: FinMap.lookup (f + (List.length Γ' - List.length Γ)) Γ' = T := by
+          rcases r with ⟨Δ, E⟩
+          simp [E]
+          assumption
+        cases T with
+        | none =>
+          simp [η_trans, Tm.up, E, K]
+        | some T =>
+          simp [η_trans, Tm.up, E, K]
+          split
+          . simp [Tm.up]
+          . simp [Tm.up]
+
+
+def Γ := [(Ty.Atom.imp .Atom).imp .Atom]
+def t := Tm.app (.var 0) (.abs $ .app (.var 1) (.abs (.var 1))) -- f (λx.(f λy.x))
+
+
+theorem N: Tm.NF Γ t Ty.Atom
+:= by
+  unfold t Γ
+  apply Tm.NF.atom
+  apply Tm.NE.app
+  . apply Tm.NE.var
+    simp
+    eq_refl
+  . apply Tm.NF.abs
+    apply Tm.NF.atom
+    apply Tm.NE.app
+    . apply Tm.NE.var
+      simp
+      eq_refl
+    . apply Tm.NF.abs
+      apply Tm.NF.atom
+      apply Tm.NE.var
+      simp
+
+
+theorem η_trans_neq_id_lemma:
+  η_trans Γ t ≠ t
+:= by
+  simp [η_trans, Γ, t]
+
+
+theorem η_trans_neq_id:
+  η.trans (Γ := Γ) ≠ η_id.trans
+:= by
+  intro E
+  replace E := congrFun E ⟨t, N⟩
+  simp [η, η_id, η_trans, t, Γ] at E
+  cases E
